Instances.lean
@@ -13,6 +13,8 @@ import Instances.Examples.VexMovMemRdiRaxFixture
 import Instances.Examples.VexStore64Example
 import Instances.ISAs.MachineISA
 import Instances.ISAs.VexSyntax
+import Instances.ISAs.VexConcrete
+import Instances.ISAs.VexLowerCore
 import Instances.ISAs.VexISA
 import Instances.ISAs.VexSummary
 import Instances.ISAs.VexBridgeCore
